Deal with mangled unicode quotes

tutorial/solutions/splitwordsScript.sml
@@ -1,1 +1,81 @@
-../splitwordsScript.sml
+(*
+  A high-level specification of words and frequencies
+*)
+
+open preamble
+     mlstringTheory
+     fsFFIPropsTheory
+
+val _ = new_theory"splitwords";
+
+val splitwords_def = Define`
+  splitwords s = tokens isSpace s`;
+(*
+EVAL ``splitwords (strlit"hello there hello how are you one two one two three")``
+*)
+
+Theorem splitwords_nil[simp]
+  `splitwords (implode "") = []` (EVAL_TAC);
+Theorem splitwords_nil_lit[simp]
+  `splitwords (strlit "") = []` (EVAL_TAC);
+
+Theorem splitwords_concat
+  `isSpace sp ⇒
+   splitwords (s1 ^ str sp ^ s2) = splitwords s1 ++ splitwords s2`
+  (rewrite_tac [GSYM strcat_assoc]
+  \\ rw[splitwords_def,mlstringTheory.tokens_append,mlstringTheory.strcat_assoc]);
+
+Theorem splitwords_concat_space
+  `isSpace sp ⇒ splitwords (s1 ^ str sp) = splitwords s1`
+  (rw[] \\ qspec_then`implode ""`mp_tac(Q.GEN`s2`splitwords_concat) \\
+  fs[mlstringTheory.strcat_thm]);
+
+Theorem splitwords_all_lines
+  `FLAT (MAP splitwords (all_lines fs fname)) =
+   splitwords (implode (THE (ALOOKUP fs.files fname)))`
+  (`isSpace #"\n"` by EVAL_TAC \\
+  rw[all_lines_def,lines_of_def,MAP_MAP_o,o_DEF,
+     GSYM mlstringTheory.str_def,splitwords_concat_space] \\
+  rw[splitwords_def,mlstringTheory.TOKENS_eq_tokens_sym] \\
+  srw_tac[ETA_ss][GSYM o_DEF,GSYM MAP_MAP_o] \\
+  simp[GSYM MAP_FLAT] \\ AP_TERM_TAC \\
+  qspec_tac(`THE (ALOOKUP fs.files fname)`,`ls`) \\
+  rw[splitlines_def]
+  >- (
+    qmatch_asmsub_abbrev_tac`NULL (LAST l)` \\
+    Q.ISPEC_THEN`l`mp_tac APPEND_FRONT_LAST \\
+    impl_tac >- rw[Abbr`l`] \\
+    fs[NULL_EQ] \\ strip_tac \\
+    `FLAT (MAP (TOKENS isSpace) (FRONT l)) = FLAT (MAP (TOKENS isSpace) l)` by (
+      pop_assum(fn th => CONV_TAC(RAND_CONV(DEPTH_CONV(REWR_CONV(SYM th))))) \\
+      simp[] \\ EVAL_TAC ) \\
+    simp[Abbr`l`] \\
+    match_mp_tac FLAT_MAP_TOKENS_FIELDS \\
+    rw[] \\ EVAL_TAC ) \\
+  match_mp_tac FLAT_MAP_TOKENS_FIELDS \\
+  rw[] \\ EVAL_TAC);
+
+val frequency_def = Define`
+  frequency s w = LENGTH (FILTER ($= w) (splitwords s))`;
+(*
+EVAL``frequency (strlit"hello there hello how are you one two one two three") (strlit"hello")``
+EVAL``frequency (strlit"hello there hello how are you one two one two three") (strlit"one")``
+EVAL``frequency (strlit"hello there hello how are you one two one two three") (strlit"three")``
+EVAL``frequency (strlit"hello there hello how are you one two one two three") (strlit"four")``
+*)
+
+Theorem frequency_nil[simp]
+  `frequency (implode "") w = 0` (EVAL_TAC);
+Theorem frequency_nil_lit[simp]
+  `frequency (strlit "") w = 0` (EVAL_TAC);
+
+Theorem frequency_concat
+  `isSpace sp ⇒
+   frequency (s1 ^ str sp ^ s2) w = frequency s1 w + frequency s2 w`
+  (rw[frequency_def,splitwords_concat,FILTER_APPEND]);
+
+Theorem frequency_concat_space
+  `isSpace sp ⇒ frequency (s1 ^ str sp) = frequency s1`
+  (rw[FUN_EQ_THM,frequency_def,splitwords_concat_space]);
+
+val _ = export_theory();
