tutorial/solutions/wordfreqProofScript.sml
@@ -1,1 +1,69 @@
-../wordfreqProofScript.sml
+open preamble
+     semanticsPropsTheory backendProofTheory x64_configProofTheory
+     wordfreqProgTheory wordfreqCompileTheory
+
+val _ = new_theory"wordfreqProof";
+
+val wordfreq_io_events_def = new_specification("wordfreq_io_events_def",["wordfreq_io_events"],
+  wordfreq_semantics |> Q.GENL[`fs`,`pname`,`fname`]
+  |> SIMP_RULE bool_ss [SKOLEM_THM,Once(GSYM RIGHT_EXISTS_IMP_THM),RIGHT_EXISTS_AND_THM]);
+
+val (wordfreq_sem,wordfreq_output) = wordfreq_io_events_def |> SPEC_ALL |> UNDISCH |> CONJ_PAIR
+val (wordfreq_not_fail,wordfreq_sem_sing) = MATCH_MP semantics_prog_Terminate_not_Fail wordfreq_sem |> CONJ_PAIR
+
+val compile_correct_applied =
+  MATCH_MP compile_correct wordfreq_compiled
+  |> SIMP_RULE(srw_ss())[LET_THM,ml_progTheory.init_state_env_thm,GSYM AND_IMP_INTRO]
+  |> C MATCH_MP wordfreq_not_fail
+  |> C MATCH_MP x64_backend_config_ok
+  |> REWRITE_RULE[wordfreq_sem_sing,AND_IMP_INTRO]
+  |> REWRITE_RULE[Once (GSYM AND_IMP_INTRO)]
+  |> C MATCH_MP (CONJ(UNDISCH x64_machine_config_ok)(UNDISCH x64_init_ok))
+  |> DISCH(#1(dest_imp(concl x64_init_ok)))
+  |> REWRITE_RULE[AND_IMP_INTRO]
+
+val wordfreq_compiled_lemma =
+  CONJ compile_correct_applied wordfreq_output
+  |> SIMP_RULE std_ss [AND_IMP_INTRO,GSYM CONJ_ASSOC]
+  |> DISCH_ALL;
+
+val compiler_output_def = Define `
+  compiler_output = (code,data,config)`;
+
+(* TODO: move  *)
+
+val get_file_contents_def = Define `
+  get_file_contents fs fname =
+    if inFS_fname fs (File fname) then
+      case ALOOKUP fs.files (File fname) of
+      | NONE => NONE
+      | SOME s => SOME (implode s)
+    else NONE`
+
+val wfFS_def = Define `
+  wfFS fs <=> fsFFIProps$wfFS fs ∧ STD_streams fs`;
+
+val x64_installed_def = Define `
+  x64_installed (c,d,conf) cbspace data_sp ffi mc ms <=>
+    is_x64_machine_config mc ∧
+    backendProof$installed c cbspace d data_sp conf.ffi_names ffi
+      (heap_regs x64_backend_config.stack_conf.reg_names) mc ms`
+
+(* -- *)
+
+Theorem wordfreq_compiled_thm
+  `wfcl [pname; fname] ∧ wfFS fs ∧ hasFreeFD fs ∧
+    (get_file_contents fs fname = SOME file_contents) ∧
+    x64_installed compiler_output cbspace data_sp (basis_ffi [pname; fname] fs) mc ms ⇒
+    ∃io_events ascii_output.
+      machine_sem mc (basis_ffi [pname; fname] fs) ms ⊆
+      extend_with_resource_limit {Terminate Success io_events} ∧
+      (extract_fs fs io_events = SOME (add_stdout fs ascii_output)) ∧
+      valid_wordfreq_output file_contents ascii_output`
+  (strip_tac
+  \\ assume_tac wordfreq_compiled_lemma
+  \\ rfs [get_file_contents_def,wfFS_def,compiler_output_def,x64_installed_def]
+  \\ asm_exists_tac \\ fs [option_case_eq]
+  \\ metis_tac [wordfreqProgTheory.wordfreq_output_spec_def]);
+
+val _ = export_theory();
