examples/compilation/x64/proofs/wordcountProofScript.sml
@@ -1,1 +1,33 @@
-../../../../tutorial/wordcountProofScript.sml
+open preamble
+     semanticsPropsTheory backendProofTheory x64_configProofTheory
+     wordcountProgTheory wordcountCompileTheory
+
+val _ = new_theory"wordcountProof";
+
+val _ = temp_clear_overloads_on"STRCAT"; (* " *)
+
+val wordcount_io_events_def = new_specification("wordcount_io_events_def",["wordcount_io_events"],
+  wordcount_semantics |> Q.GENL[`cl`,`fs`,`contents`,`fs'`]
+  |> SIMP_RULE bool_ss [SKOLEM_THM,Once(GSYM RIGHT_EXISTS_IMP_THM)]);
+
+val (wordcount_sem,wordcount_output) = wordcount_io_events_def |> SPEC_ALL |> UNDISCH |> CONJ_PAIR
+val (wordcount_not_fail,wordcount_sem_sing) = MATCH_MP semantics_prog_Terminate_not_Fail wordcount_sem |> CONJ_PAIR
+
+val compile_correct_applied =
+  MATCH_MP compile_correct wordcount_compiled
+  |> SIMP_RULE(srw_ss())[LET_THM,ml_progTheory.init_state_env_thm,GSYM AND_IMP_INTRO]
+  |> C MATCH_MP wordcount_not_fail
+  |> C MATCH_MP x64_backend_config_ok
+  |> REWRITE_RULE[wordcount_sem_sing,AND_IMP_INTRO]
+  |> REWRITE_RULE[Once (GSYM AND_IMP_INTRO)]
+  |> C MATCH_MP (CONJ(UNDISCH x64_machine_config_ok)(UNDISCH x64_init_ok))
+  |> DISCH(#1(dest_imp(concl x64_init_ok)))
+  |> REWRITE_RULE[AND_IMP_INTRO]
+
+val wordcount_compiled_thm =
+  CONJ compile_correct_applied wordcount_output
+  |> DISCH_ALL
+  |> check_thm
+  |> curry save_thm "wordcount_compiled_thm";
+
+val _ = export_theory();
