examples/compilation/x64/wordcountCompileScript.sml
@@ -1,1 +1,17 @@
-../../../tutorial/wordcountCompileScript.sml
+(*
+  Compile the wordcount program to machine code by evaluation of the compiler
+  in the logic.
+*)
+
+open preamble wordcountProgTheory compilationLib
+
+val _ = new_theory"wordcountCompile";
+
+val wordcount_compiled = save_thm("wordcount_compiled",
+  compile_x64
+    1000 (* stack size in MB *)
+    1000 (* heap size in MB *)
+    "wordcount"
+    wordcount_prog_def);
+
+val _ = export_theory();
