tutorial/solutions/wordfreqCompileScript.sml
@@ -1,1 +1,17 @@
-../wordfreqCompileScript.sml
+(*
+  Compile the wordfreq program to machine code by evaluation of the compiler in
+  the logic.
+*)
+
+open preamble wordfreqProgTheory compilationLib
+
+val _ = new_theory"wordfreqCompile";
+
+val wordfreq_compiled = save_thm("wordfreq_compiled",
+  compile_x64
+    1000 (* stack size in MB *)
+    1000 (* heap size in MB *)
+    "wordfreq"
+    wordfreq_prog_def);
+
+val _ = export_theory();
